Base.v
@@ -4,6 +4,8 @@ Require Export Coq.Logic.FunctionalExtensionality.
 Require Export List.
 Export ListNotations.
 
+Global Set Universe Polymorphism.
+
 Definition id {A : Type} := fun x : A => x.
 
 Notation "f .> g" := (compose g f) (at level 40).
