MonadComp/Monad.v
@@ -177,14 +177,14 @@ Proof.
   intros. unfold join, bind, compose.
   cut (((fun _ : unit => ma) >=> f) = ((fun _ : unit => fmap f ma) >=> id)).
     intro. rewrite H. reflexivity.
-    Print Monad. unfold id. extensionality x. destruct x.
+    unfold id. extensionality x. destruct x.
 Abort. (* TODO *)
 
 Theorem fmap_ret :
   forall (M : Type -> Type) (inst : Monad M) (A B : Type) (f : A -> B) (x : A),
     fmap f (ret x) = ret (f x).
 Proof.
-  intros. Print Monad. 
+  intros.
 Admitted. (* TODO *)
 
 Theorem ret_bind :
