MonadJoin/Lazy3.v
@@ -1,0 +1,54 @@
+Add Rec LoadPath "/home/Zeimer/Code/Coq".
+
+Require Import HSLib.Base.
+Require Export HSLib.MonadJoin.Monad.
+
+Definition Lazy (A : Type) : Type := unit -> A.
+
+Definition delay {A : Type} (a : A) : Lazy A :=
+  fun _ => a.
+
+Definition force {A : Type} (la : Lazy A) : A :=
+  la tt.
+
+Definition fmap_Lazy {A B : Type} (f : A -> B) (la : Lazy A) : Lazy B :=
+  fun _ => f (la tt).
+
+Instance FunctorLazy : Functor Lazy :=
+{
+    fmap := @fmap_Lazy;
+}.
+Proof.
+  intro. unfold id, fmap_Lazy.
+    extensionality la. extensionality u. destruct u. reflexivity.
+  intros. unfold compose, fmap_Lazy.
+    extensionality la. reflexivity.
+Defined.
+
+Definition ret_Lazy {A : Type} (a : A) : Lazy A :=
+  fun _ => a.
+
+Definition bind_Lazy
+  {A B : Type} (la : Lazy A) (f : A -> Lazy B) : Lazy B :=
+    f (la tt).
+
+Definition join_Lazy {A : Type} (lla : Lazy (Lazy A)) : Lazy A :=
+  lla tt.
+
+Instance MonadLazy : Monad Lazy :=
+{
+    ret := @ret_Lazy;
+    join := @join_Lazy;
+}.
+Proof.
+  reflexivity.
+  cbn. intros. unfold compose, ret_Lazy, join_Lazy, fmap_Lazy.
+    extensionality la. extensionality u. destruct u. reflexivity.
+Defined.
+
+Eval lazy in
+  delay 5 >>= fun n : nat =>
+  delay 2 >>= fun m : nat => delay (n * m).
+
+Eval lazy in
+  delay 42 >>= fun n : nat => delay (2 * n).
