Parser/MonadicParserCombinators.v
@@ -1,0 +1,344 @@
+(** * Monadic Parser Combinators *)
+
+(** This file is a Coq translation of code taken from the paper "Monadic
+    Parser Combinators" by Graham Hutton and Erik Meijer. *)
+
+Require Import Ascii.
+Require Import String.
+
+Require Import List.
+Import ListNotations.
+
+(** ** 1 Introduction *)
+
+(** ** 2 Combinator parsers *)
+
+(** *** 2.1 The type of parsers *)
+
+Definition Parser (A : Type) : Type := string -> list (A * string).
+
+(** *** 2.2 Primitive parsers *)
+
+Definition result {A : Type} (x : A) : Parser A :=
+  fun input : string => [(x, input)].
+
+Definition zero {A : Type} : Parser A :=
+  fun _ => [].
+
+Definition item {A : Type} : Parser ascii :=
+  fun input : string =>
+  match input with
+      | EmptyString => []
+      | String c cs => [(c, cs)]
+  end.
+
+(** *** 2.3 Parser combinators *)
+
+Fixpoint join {A : Type} (lla : list (list A)) : list A :=
+match lla with
+    | [] => []
+    | l :: ls => l ++ join ls
+end.
+
+Definition bind
+  {A B : Type} (p : Parser A) (f : A -> Parser B) : Parser B :=
+  fun input : string =>
+    join (map (fun x : A * string =>
+      let '(v, input') := x in f v input') (p input)).
+
+Definition seq
+  {A B : Type} (pa : Parser A) (pb : Parser B) : Parser (A * B) :=
+    bind pa (fun a : A =>
+    bind pb (fun b : B =>
+      result (a, b))).
+
+Definition sat (p : ascii -> bool) : Parser ascii :=
+  bind (@item ascii) (fun c : ascii =>
+    if p c then result c else zero).
+
+Require Import Bool.
+
+Definition ascii_eqb (x y : ascii) : bool :=
+  if ascii_dec x y then true else false.
+
+Lemma ascii_eqb_spec :
+  forall x y : ascii, reflect (x = y) (ascii_eqb x y).
+Proof.
+  intros. unfold ascii_eqb.
+  destruct (ascii_dec x y); firstorder.
+Qed.
+
+Definition char (c : ascii) : Parser ascii :=
+  sat (fun c' : ascii => ascii_eqb c c').
+
+Open Scope char_scope.
+Open Scope string_scope.
+
+Require Import Arith.
+
+Definition digit : Parser ascii :=
+  sat (fun c : ascii =>
+    Nat.leb 48 (nat_of_ascii c) && Nat.leb (nat_of_ascii c) 57).
+
+Definition lower : Parser ascii :=
+  sat (fun c : ascii =>
+    Nat.leb 97 (nat_of_ascii c) && Nat.leb (nat_of_ascii c) 122).
+
+Compute nat_of_ascii "A".
+Compute nat_of_ascii "Z".
+
+Definition upper : Parser ascii :=
+  sat (fun c : ascii =>
+    Nat.leb 65 (nat_of_ascii c) && Nat.leb (nat_of_ascii c) 90).
+
+Compute bind lower (fun x =>
+        bind lower (fun y =>
+          result (String x (String y EmptyString)))) "hello".
+
+Open Scope list_scope.
+
+Definition plus {A : Type} (p1 p2 : Parser A) : Parser A :=
+  fun input : string => (p1 input) ++ (p2 input).
+
+Definition letter : Parser ascii :=
+  plus lower upper.
+
+Definition alphanum : Parser ascii :=
+  plus letter digit.
+
+(** All words of length less than or equal to n. *)
+Fixpoint words (n : nat) : Parser string :=
+match n with
+    | 0 => result ""
+    | S n' => plus
+                (bind letter (fun c =>
+                 bind (words n') (fun cs =>
+                   result (String c cs))))
+                (result "")
+end.
+
+(** A word of any length. *)
+Definition word : Parser string :=
+  fun input : string => words (String.length input) input.
+
+(** ** 3 Parsers and monads *)
+
+(** *** 3.1 The parser monad *)
+
+(* TODO *)
+
+(** *** 3.2 Monad comprehension syntax *)
+
+Fixpoint str (s : string) : Parser string :=
+(*  fun input : string =>*)
+match s with
+    | "" => result ""
+    | String c cs =>
+        bind (char c) (fun _ => bind (str cs) (fun _ => result (String c cs)))
+end.
+
+Compute str "abc" "abcd".
+
+(** ** 4 Combinators for repetition *)
+
+(** *** 4.1 Simple repetition *)
+
+Fixpoint many' {A : Type} (n : nat) (p : Parser A) : Parser (list A) :=
+match n with
+    | 0 => result []
+    | S n' => plus
+                (bind p (fun h =>
+                 bind (many' n' p) (fun t =>
+                   result (h :: t))))
+                (result [])
+end.
+
+Open Scope char_scope.
+
+Compute many' 5 letter "asdsd"%string.
+
+Definition many {A : Type} (p : Parser A) : Parser (list A) :=
+  fun input : string => many' (String.length input) p input.
+
+Compute many digit "123"%string.
+
+Definition fmap {A B : Type} (f : A -> B) (p : Parser A) : Parser B :=
+  fun input : string =>
+    map (fun p => (f (fst p), snd p)) (p input).
+
+Fixpoint toString (l : list ascii) : string :=
+match l with
+    | [] => ""
+    | c :: cs => String c (toString cs)
+end.
+
+Definition word' : Parser string :=
+  fmap toString (many letter).
+
+Compute word "abc"%string.
+Compute word' "abc"%string.
+
+Definition ident : Parser string :=
+  bind lower (fun c =>
+  bind (fmap toString (many alphanum)) (fun cs => result (String c cs))).
+
+Compute ident "wut123"%string.
+
+Definition many1 {A : Type} (p : Parser A) : Parser (list A) :=
+  bind p (fun h =>
+  bind (many p) (fun t =>
+    result (h :: t))).
+
+Compute many1 (char "a") "aaab"%string.
+
+Fixpoint eval (cs : list ascii) : nat :=
+match cs with
+    | [] => 0
+    | c :: cs' => nat_of_ascii c - 48 + 10 * eval cs'
+end.
+
+Definition parseNat : Parser nat :=
+  fmap (fun l => eval (rev l)) (many1 digit).
+
+Compute parseNat "123"%string.
+
+Require Import ZArith.
+
+Definition parseNeg : Parser nat :=
+  fmap (fun l => eval (rev l))
+    (bind (char "-") (fun _ => many1 digit)).
+
+Definition parseZ : Parser Z :=
+  plus
+    (fmap Z_of_nat parseNat)
+    (fmap (fun n => Z.sub 0%Z (Z_of_nat n)) parseNeg).
+
+Compute parseZ "-12345"%string.
+
+Definition parseSign : Parser (Z -> Z) :=
+(*  fmap (fun l => match l with | [] => [] | h :: _ => [h] end)*)
+    plus
+      (bind (char "-") (fun _ =>
+      (result (fun k => Z.sub 0%Z k))))
+      (result id).
+
+Definition parseZ' : Parser Z :=
+  bind parseSign (fun f =>
+  bind parseNat (fun n =>
+    result (f (Z_of_nat n)))).
+
+Compute parseZ' "-12345"%string.
+
+(** *** 4.2 Repetition with separators *)
+
+Definition sepby1 {A B : Type} (p : Parser A) (sep : Parser B) : 
+  Parser (list A) :=
+    bind p (fun h =>
+    bind (many (bind sep (fun _ => p))) (fun t =>
+      result (h :: t))).
+
+Definition bracket {A B C : Type}
+  (open : Parser A) (content : Parser B) (close : Parser C) : Parser B :=
+    bind open (fun _ =>
+    bind content (fun res =>
+    bind close (fun _ =>
+      result res))).
+
+Definition ints : Parser (list Z) :=
+  bracket (char "[") (sepby1 parseZ (char ",")) (char "]").
+
+Compute ints "[1,2]"%string.
+
+Definition sepby {A B : Type}
+  (item : Parser A) (sep : Parser B) : Parser (list A) :=
+    plus (sepby1 item sep) (result []).
+
+(** *** 4.3 Repetition with meaningful separators *)
+
+(**
+    expr    ::= expr addop factor | factor
+    addop   ::= + | -
+    factor  ::= nat | ( expr )
+*)
+
+Fixpoint exprn (n : nat) : Parser Z :=
+match n with
+    | 0 => result 42%Z
+    | S n' =>
+        let
+          addop := plus (bind (char "+") (fun _ => result Z.add))
+                        (bind (char "-") (fun _ => result Z.sub))
+        in let
+          factor := plus parseZ
+                         (bracket (char "(") (exprn n') (char ")"))
+        in
+          plus
+            (bind (exprn n') (fun x =>
+             bind addop (fun op =>
+             bind factor (fun y =>
+               result (op x y)))))
+            factor
+end.
+
+Definition expr : Parser Z :=
+  fun input : string => exprn (String.length input) input.
+
+Compute expr "2+2"%string.
+
+Compute expr "0-5)"%string.
+
+Notation "a |: b" := (plus a b) (at level 50).
+
+Definition chainl1
+  {A : Type} (p : Parser A) (p_op : Parser (A -> A -> A)) : Parser A :=
+    bind p (fun start =>
+    bind (many (bind p_op (fun op =>
+                bind p (fun arg =>
+                  result (op, arg)))))
+         (fun l => result (fold_left (fun x p => fst p x (snd p)) l start))).
+
+Fixpoint exprn'' (n : nat) : Parser Z :=
+match n with
+    | 0 => result 0%Z
+    | S n' =>
+        let
+          op := bind (char "+") (fun _ => result Z.add) |:
+                bind (char "-") (fun _ => result Z.sub)
+        in let
+          factor := parseZ |: bracket (char "(") (exprn'' n') (char ")")
+        in
+          chainl1 factor op
+end.
+
+Definition expr'' : Parser Z :=
+  fun input : string => exprn'' (String.length input) input.
+
+Compute expr'' "3-2"%string.
+
+Definition ops
+  {A B : Type} (start : Parser A * B) (l : list (Parser A * B)) : Parser B :=
+match l with
+    | [] => let '(p, op) := start in bind p (fun _ => result op)
+    | h :: t =>
+        fold_right plus (bind (fst start) (fun _ => result (snd start)))
+          (map (fun x => bind (fst x) (fun _ => result (snd x))) l)
+end.
+
+Fixpoint exprn3 (n : nat) : Parser Z :=
+match n with
+    | 0 => result 0%Z
+    | S n' =>
+        let
+          op := ops (char "+", Z.add) [(char "-", Z.sub)]
+        in let
+          factor := parseZ |: bracket (char "(") (exprn3 n') (char ")")
+        in
+          chainl1 factor op
+end.
+
+Definition expr3 : Parser Z :=
+  fun input : string => exprn3 (String.length input) input.
+
+Compute expr'' "1-(2-(3-4)-5)"%string.
+
+(* TODO: chainl1 alternative and chainr1 *)
