clean.sh
@@ -1,0 +1,5 @@
+#!/bin/bash
+make clean
+rm *vo *glob *v.d *~ .*.vo.aux
+rm */*vo */*glob */*v.d */*~ */*.vo.aux
+rm */*/*vo */*/*glob */*/*v.d */*/*~ */*/*.vo.aux
