make_makefile.sh
@@ -1,0 +1,7 @@
+#!/bin/sh
+
+#coq_makefile -R "." HSLib -o makefile Base.v Alternative/**v Applicative Functor Instances InstancesT MonadBind MonadComp MonadJoin MonadPlus MonadTrans
+
+coq_makefile -R "." HSLib -o makefile **v */**v
+
+#coq_makefile -R "." RandomCoqCode -o makefile RCCBase.v Reflection/**v Sorting/**v Structures/**v Trash/**v Trees/**v
